Reorganize reduction-consistent proof theory and semantics. Start adding type classes for semantics and kripke models.

PropositionalLogic/ClassicalPropositionalLogic.v
@@ -8,13 +8,12 @@ Require Import Logic.PropositionalLogic.MinimunPropositionalLogic.
 Local Open Scope logic_base.
 Local Open Scope PropositionalLogic.
 
-Class ClassicalPropositionalLogic (L: Language) {nL: NormalLanguage L} {pL: PropositionalLanguage L} (Gamma: ProofTheory L) {mpGamma: MinimunPropositionalLogic L Gamma} := {
-  syntactic_reduction_rule: forall x y, @reduce _ MendelsonReduction x y -> (|-- x <-> |-- y);
+Class ClassicalPropositionalLogic (L: Language) {nL: NormalLanguage L} {pL: PropositionalLanguage L} (Gamma: ProofTheory L) {mpGamma: MinimunPropositionalLogic L Gamma} {rcGamma: ReductionConsistentProofTheory MendelsonReduction Gamma} := {
   axiom3: forall x y, |-- ((~~ y --> x) --> (~~ y --> ~~ x) --> y);
   true_provable: provable TT
 }.
 
-Lemma axiom3_derivable: forall {L: Language} {nL: NormalLanguage L} {pL: PropositionalLanguage L} {Gamma: ProofTheory L} {nGamma: NormalProofTheory L Gamma} {mpGamma: MinimunPropositionalLogic L Gamma} {cpGamma: ClassicalPropositionalLogic L Gamma} (Phi: context) (x y: expr),
+Lemma axiom3_derivable: forall {L: Language} {nL: NormalLanguage L} {pL: PropositionalLanguage L} {Gamma: ProofTheory L} {nGamma: NormalProofTheory L Gamma} {mpGamma: MinimunPropositionalLogic L Gamma} {rcGamma: ReductionConsistentProofTheory MendelsonReduction Gamma} {cpGamma: ClassicalPropositionalLogic L Gamma} (Phi: context) (x y: expr),
   Phi |-- (~~ x --> y) --> (~~ x --> ~~ y) --> x.
 Proof.
   intros.
@@ -24,7 +23,7 @@ Proof.
   intros ? [].
 Qed.
 
-Lemma contradiction_rule: forall {L: Language} {nL: NormalLanguage L} {pL: PropositionalLanguage L} {Gamma: ProofTheory L} {nGamma: NormalProofTheory L Gamma} {mpGamma: MinimunPropositionalLogic L Gamma} {cpGamma: ClassicalPropositionalLogic L Gamma} (Phi: context) (x y: expr),
+Lemma contradiction_rule: forall {L: Language} {nL: NormalLanguage L} {pL: PropositionalLanguage L} {Gamma: ProofTheory L} {nGamma: NormalProofTheory L Gamma} {mpGamma: MinimunPropositionalLogic L Gamma} {rcGamma: ReductionConsistentProofTheory MendelsonReduction Gamma} {cpGamma: ClassicalPropositionalLogic L Gamma} (Phi: context) (x y: expr),
   Phi |-- ~~ x ->
   Phi |-- x ->
   Phi |-- y.
@@ -38,7 +37,7 @@ Proof.
   auto.
 Qed.
 
-Lemma double_negp_add: forall {L: Language} {nL: NormalLanguage L} {pL: PropositionalLanguage L} {Gamma: ProofTheory L} {nGamma: NormalProofTheory L Gamma} {mpGamma: MinimunPropositionalLogic L Gamma} {cpGamma: ClassicalPropositionalLogic L Gamma} (Phi: context) (x: expr),
+Lemma double_negp_add: forall {L: Language} {nL: NormalLanguage L} {pL: PropositionalLanguage L} {Gamma: ProofTheory L} {nGamma: NormalProofTheory L Gamma} {mpGamma: MinimunPropositionalLogic L Gamma} {rcGamma: ReductionConsistentProofTheory MendelsonReduction Gamma} {cpGamma: ClassicalPropositionalLogic L Gamma} (Phi: context) (x: expr),
   Phi |-- ~~ (~~ x) --> x.
 Proof.
   intros.
@@ -49,7 +48,7 @@ Proof.
   auto.
 Qed.
 
-Lemma double_negp_elim: forall {L: Language} {nL: NormalLanguage L} {pL: PropositionalLanguage L} {Gamma: ProofTheory L} {nGamma: NormalProofTheory L Gamma} {mpGamma: MinimunPropositionalLogic L Gamma} {cpGamma: ClassicalPropositionalLogic L Gamma} (Phi: context) (x: expr),
+Lemma double_negp_elim: forall {L: Language} {nL: NormalLanguage L} {pL: PropositionalLanguage L} {Gamma: ProofTheory L} {nGamma: NormalProofTheory L Gamma} {mpGamma: MinimunPropositionalLogic L Gamma} {rcGamma: ReductionConsistentProofTheory MendelsonReduction Gamma} {cpGamma: ClassicalPropositionalLogic L Gamma} (Phi: context) (x: expr),
   Phi |-- x --> ~~ ~~ x.
 Proof.
   intros.
@@ -60,7 +59,7 @@ Proof.
   auto.
 Qed.
 
-Lemma contrapositivePP: forall {L: Language} {nL: NormalLanguage L} {pL: PropositionalLanguage L} {Gamma: ProofTheory L} {nGamma: NormalProofTheory L Gamma} {mpGamma: MinimunPropositionalLogic L Gamma} {cpGamma: ClassicalPropositionalLogic L Gamma} Phi (x y: expr),
+Lemma contrapositivePP: forall {L: Language} {nL: NormalLanguage L} {pL: PropositionalLanguage L} {Gamma: ProofTheory L} {nGamma: NormalProofTheory L Gamma} {mpGamma: MinimunPropositionalLogic L Gamma} {rcGamma: ReductionConsistentProofTheory MendelsonReduction Gamma} {cpGamma: ClassicalPropositionalLogic L Gamma} Phi (x y: expr),
   Phi |-- ~~ y --> ~~ x ->
   Phi |-- x --> y.
 Proof.
@@ -75,7 +74,7 @@ Proof.
   auto.
 Qed.
 
-Lemma contrapositiveNN: forall {L: Language} {nL: NormalLanguage L} {pL: PropositionalLanguage L} {Gamma: ProofTheory L} {nGamma: NormalProofTheory L Gamma} {mpGamma: MinimunPropositionalLogic L Gamma} {cpGamma: ClassicalPropositionalLogic L Gamma} Phi (x y: expr),
+Lemma contrapositiveNN: forall {L: Language} {nL: NormalLanguage L} {pL: PropositionalLanguage L} {Gamma: ProofTheory L} {nGamma: NormalProofTheory L Gamma} {mpGamma: MinimunPropositionalLogic L Gamma} {rcGamma: ReductionConsistentProofTheory MendelsonReduction Gamma} {cpGamma: ClassicalPropositionalLogic L Gamma} Phi (x y: expr),
   Phi |-- y --> x ->
   Phi |-- ~~ x --> ~~ y.
 Proof.
@@ -87,7 +86,7 @@ Proof.
   apply derivable_weaken1; eauto.
 Qed.
 
-Lemma contrapositiveNP: forall {L: Language} {nL: NormalLanguage L} {pL: PropositionalLanguage L} {Gamma: ProofTheory L} {nGamma: NormalProofTheory L Gamma} {mpGamma: MinimunPropositionalLogic L Gamma} {cpGamma: ClassicalPropositionalLogic L Gamma} Phi (x y: expr),
+Lemma contrapositiveNP: forall {L: Language} {nL: NormalLanguage L} {pL: PropositionalLanguage L} {Gamma: ProofTheory L} {nGamma: NormalProofTheory L Gamma} {mpGamma: MinimunPropositionalLogic L Gamma} {rcGamma: ReductionConsistentProofTheory MendelsonReduction Gamma} {cpGamma: ClassicalPropositionalLogic L Gamma} Phi (x y: expr),
   Phi |-- ~~ y --> x ->
   Phi |-- ~~ x --> y.
 Proof.
@@ -98,7 +97,7 @@ Proof.
   apply deduction_theorem; auto.
 Qed.
 
-Lemma contrapositivePN: forall {L: Language} {nL: NormalLanguage L} {pL: PropositionalLanguage L} {Gamma: ProofTheory L} {nGamma: NormalProofTheory L Gamma} {mpGamma: MinimunPropositionalLogic L Gamma} {cpGamma: ClassicalPropositionalLogic L Gamma} Phi (x y: expr),
+Lemma contrapositivePN: forall {L: Language} {nL: NormalLanguage L} {pL: PropositionalLanguage L} {Gamma: ProofTheory L} {nGamma: NormalProofTheory L Gamma} {mpGamma: MinimunPropositionalLogic L Gamma} {rcGamma: ReductionConsistentProofTheory MendelsonReduction Gamma} {cpGamma: ClassicalPropositionalLogic L Gamma} Phi (x y: expr),
   Phi |-- y --> ~~ x ->
   Phi |-- x --> ~~ y.
 Proof.
@@ -109,7 +108,7 @@ Proof.
   apply derivable_weaken1; auto.
 Qed.
 
-Lemma assum_exclude_middle: forall {L: Language} {nL: NormalLanguage L} {pL: PropositionalLanguage L} {Gamma: ProofTheory L} {nGamma: NormalProofTheory L Gamma} {mpGamma: MinimunPropositionalLogic L Gamma} {cpGamma: ClassicalPropositionalLogic L Gamma} (Phi: context) (x y: expr),
+Lemma assum_exclude_middle: forall {L: Language} {nL: NormalLanguage L} {pL: PropositionalLanguage L} {Gamma: ProofTheory L} {nGamma: NormalProofTheory L Gamma} {mpGamma: MinimunPropositionalLogic L Gamma} {rcGamma: ReductionConsistentProofTheory MendelsonReduction Gamma} {cpGamma: ClassicalPropositionalLogic L Gamma} (Phi: context) (x y: expr),
   Phi |-- ~~ x --> y ->
   Phi |-- x --> y ->
   Phi |-- y.
@@ -123,7 +122,7 @@ Proof.
   auto.
 Qed.
 
-Lemma aux_classic_theorem05: forall {L: Language} {nL: NormalLanguage L} {pL: PropositionalLanguage L} {Gamma: ProofTheory L} {nGamma: NormalProofTheory L Gamma} {mpGamma: MinimunPropositionalLogic L Gamma} {cpGamma: ClassicalPropositionalLogic L Gamma} (Phi: context) (x: expr),
+Lemma aux_classic_theorem05: forall {L: Language} {nL: NormalLanguage L} {pL: PropositionalLanguage L} {Gamma: ProofTheory L} {nGamma: NormalProofTheory L Gamma} {mpGamma: MinimunPropositionalLogic L Gamma} {rcGamma: ReductionConsistentProofTheory MendelsonReduction Gamma} {cpGamma: ClassicalPropositionalLogic L Gamma} (Phi: context) (x: expr),
   Phi |-- ~~ x --> FF ->
   Phi |-- x.
 Proof.
@@ -133,12 +132,11 @@ Proof.
   1: rewrite derivable_provable; exists nil; split; [auto | apply true_provable].
   eapply derivable_modus_ponens; eauto.
   rewrite derivable_provable; exists nil; split; [auto |].
-  simpl; eapply syntactic_reduction_rule.
+  simpl; eapply provable_reduce.
   + apply imp_reduce; [| apply reduce_refl].
     apply imp_reduce; [| apply reduce_refl].
     apply neg_reduce.
     apply reduce_step.
-    eapply (propag_reduce_spec _ _ _ nil).
     right; right; constructor.
   + simpl; clear H.
     pose proof imp_trans_strong TT (~~ ~~ TT) x.
@@ -147,7 +145,7 @@ Proof.
     apply double_negp_elim.
 Qed.
 
-Lemma MCS_nonelement_inconsistent: forall {L: Language} {nL: NormalLanguage L} {pL: PropositionalLanguage L} {Gamma: ProofTheory L} {nGamma: NormalProofTheory L Gamma} {mpGamma: MinimunPropositionalLogic L Gamma} {cpGamma: ClassicalPropositionalLogic L Gamma} (Phi: context),
+Lemma MCS_nonelement_inconsistent: forall {L: Language} {nL: NormalLanguage L} {pL: PropositionalLanguage L} {Gamma: ProofTheory L} {nGamma: NormalProofTheory L Gamma} {mpGamma: MinimunPropositionalLogic L Gamma} {rcGamma: ReductionConsistentProofTheory MendelsonReduction Gamma} {cpGamma: ClassicalPropositionalLogic L Gamma} (Phi: context),
   maximal_consistent Phi ->
   (forall x: expr, ~ Phi x <-> Phi |-- x --> FF).
 Proof.
@@ -166,7 +164,7 @@ Proof.
     destruct H; auto.
 Qed.
 
-Lemma MCS_negp_iff: forall {L: Language} {nL: NormalLanguage L} {pL: PropositionalLanguage L} {Gamma: ProofTheory L} {nGamma: NormalProofTheory L Gamma} {mpGamma: MinimunPropositionalLogic L Gamma} {cpGamma: ClassicalPropositionalLogic L Gamma} (Phi: context),
+Lemma MCS_negp_iff: forall {L: Language} {nL: NormalLanguage L} {pL: PropositionalLanguage L} {Gamma: ProofTheory L} {nGamma: NormalProofTheory L Gamma} {mpGamma: MinimunPropositionalLogic L Gamma} {rcGamma: ReductionConsistentProofTheory MendelsonReduction Gamma} {cpGamma: ClassicalPropositionalLogic L Gamma} (Phi: context),
   maximal_consistent Phi ->
   (forall x: expr, Phi (~~ x) <-> ~ Phi x).
 Proof.
@@ -187,17 +185,16 @@ Proof.
       eapply derivable_modus_ponens; eauto.
       rewrite derivable_provable; exists nil.
       split; [auto | simpl].
-      eapply syntactic_reduction_rule.
+      eapply provable_reduce.
       * apply imp_reduce; [| apply reduce_refl].
         apply imp_reduce; [apply reduce_refl |].
         apply reduce_step.
-        eapply (propag_reduce_spec _ _ _ nil).
         right; right; constructor.
       * simpl.
         apply imp_refl.
 Qed.
 
-Lemma MCS_impp_iff: forall {L: Language} {nL: NormalLanguage L} {pL: PropositionalLanguage L} {Gamma: ProofTheory L} {nGamma: NormalProofTheory L Gamma} {mpGamma: MinimunPropositionalLogic L Gamma} {cpGamma: ClassicalPropositionalLogic L Gamma} (Phi: context),
+Lemma MCS_impp_iff: forall {L: Language} {nL: NormalLanguage L} {pL: PropositionalLanguage L} {Gamma: ProofTheory L} {nGamma: NormalProofTheory L Gamma} {mpGamma: MinimunPropositionalLogic L Gamma} {rcGamma: ReductionConsistentProofTheory MendelsonReduction Gamma} {cpGamma: ClassicalPropositionalLogic L Gamma} (Phi: context),
   maximal_consistent Phi ->
   (forall x y: expr, Phi (x --> y) <-> (Phi x -> Phi y)).
 Proof.
@@ -217,14 +214,6 @@ Proof.
     - rewrite MCS_element_derivable in H0 |- * by auto.
       pose proof axiom1_derivable Phi y x.
       apply (derivable_modus_ponens _ y); auto.
-Qed.
-
-Lemma classic_mendelson_consistent: forall {L: Language} {nL: NormalLanguage L} {pL: PropositionalLanguage L} {Gamma: ProofTheory L} {nGamma: NormalProofTheory L Gamma} {mpGamma: MinimunPropositionalLogic L Gamma} {cpGamma: ClassicalPropositionalLogic L Gamma}, reduction_consistent_prooftheory MendelsonReduction Gamma.
-Proof.
-  intros.
-  apply reduction_consistent_prooftheory_from_provable; auto.
-  hnf; intros.
-  apply syntactic_reduction_rule; auto.
 Qed.
 
 Module ClassicalPropositionalLogic.
@@ -260,12 +249,16 @@ Proof.
   + apply axiom2.
 Qed.
 
+Instance rcG: ReductionConsistentProofTheory MendelsonReduction G.
+Proof.
+  hnf; intros; split.
+  + apply syntactic_reduction_rule1; auto.
+  + apply syntactic_reduction_rule2; auto.
+Qed.
+
 Instance cpG: ClassicalPropositionalLogic L G.
 Proof.
   constructor.
-  + split.
-    - apply syntactic_reduction_rule1; auto. 
-    - apply syntactic_reduction_rule2; auto. 
   + apply axiom3.
   + apply true_provable.
 Qed.
