HenkinCompleteness.v
@@ -5,9 +5,7 @@ Require Import Omega.
 
 Local Open Scope logic_base.
 
-Lemma truth_lemma_from_syntactic_reduction {L: Language} (R: SyntacticReduction L) {sR: NormalSyntacticReduction L R} (SM: Semantics L) (Gamma: ProofTheory L):
-  reduction_consistent_prooftheory R Gamma ->
-  reduction_consistent_semantics R SM ->
+Lemma truth_lemma_from_syntactic_reduction {L: Language} {nL: NormalLanguage L} (R: SyntacticReduction L) {sR: NormalSyntacticReduction L R} (SM: Semantics L) {rcSM: ReductionConsistentSemantics R SM} (Gamma: ProofTheory L) {nGamma: NormalProofTheory L Gamma} {rcGamma: ReductionConsistentProofTheory R Gamma}:
   forall (canonical_model: model) (Phi: context),
     (forall x, Phi x <-> Phi |-- x) ->
     (forall x: expr, normal_form x -> (canonical_model |= x <-> Phi x)) ->
@@ -15,12 +13,11 @@ Lemma truth_lemma_from_syntactic_reduction {L: Language} (R: SyntacticReduction 
 Proof.
   intros.
   destruct (reduce_to_norm x) as [y [? ?]].
-  specialize (H2 y H4).
-  destruct H as [_ ?];
-  specialize (H Phi Phi x y (context_reduce_refl _) H3).
-  specialize (H0 x y canonical_model H3).
-  pose proof H1 x.
-  pose proof H1 y.
+  specialize (H0 y H2).
+  specialize (derivable_reduce Phi Phi x y (context_reduce_refl _) H1).
+  specialize (sat_reduce x y canonical_model H1).
+  pose proof H x.
+  pose proof H y.
   tauto.
 Qed.
 
